show typing of memcpy

theories/lang/memcpy.v
@@ -7,7 +7,7 @@ Definition memcpy : val :=
     if: "len" ≤ #0 then #()
     else "dst" <- !"src";;
          "memcpy" ["dst" +ₗ #1 ; "len" - #1 ; "src" +ₗ #1].
-Opaque memcpy.
+Global Opaque memcpy.
 
 Notation "e1 <-{ n } ! e2" := (App memcpy [e1%E ; Lit (LitInt n) ; e2%E])
   (at level 80, n at next level, format "e1  <-{ n }  ! e2") : expr_scope.
